Merged the two implementations of red-black trees. Moved some red-black tree theorems to RedblackSort.v. Proved some missing theorems about height-balanced BSTs. Proved Elem_intersection, although using some lemmas which are still Admitted.

DS/BST/HeightBalanced.v
@@ -10,59 +10,65 @@ match t with
     | N h _ _ _ => h
 end.
 
-Definition balance {A : Type} (l : Tree A) (v : A) (r : Tree A) : Tree A :=
+Definition prebalance {A : Type} (l : Tree A) (v : A) (r : Tree A) : Tree A :=
   N (1 + max (height l) (height r)) l v r.
 
 Function rotateLR {A : Type} (t : Tree A) : Tree A :=
 match t with
-    | N _ (N _ a y b) x c => balance a y (balance b x c)
+    | N _ (N _ a y b) x c => prebalance a y (prebalance b x c)
     | _ => t
 end.
 
 Function rotateRL {A : Type} (t : Tree A) : Tree A :=
 match t with
-    | N _ a x (N _ b y c) => balance (balance a x b) y c
+    | N _ a x (N _ b y c) => prebalance (prebalance a x b) y c
     | _ => t
 end.
 
-Function rebalance {A : Type} (l : Tree A) (v : A) (r : Tree A) : Tree A :=
+Function balance {A : Type} (l : Tree A) (v : A) (r : Tree A) : Tree A :=
 match height l <?> height r with
     | Lt =>
         match r with
-            | N _ a x b => balance (balance l x a) v b
-            | _ => balance l v r
+            | N _ a x b => prebalance (prebalance l v a) x b
+            | _ => prebalance l v r
         end
-    | Eq => balance l v r
+    | Eq => prebalance l v r
     | Gt =>
         match l with
-            | N _ a x b => balance a v (balance b x r)
-            | _ => balance l v r
+            | N _ a x b => prebalance a x (prebalance b v r)
+            | _ => prebalance l v r
         end
 end.
 
-Function insert {A : Ord} (x : A) (t : Tree A) : Tree A :=
+Function insert {A : Type} (leb : A -> A -> bool) (x : A) (t : Tree A) : Tree A :=
 match t with
     | E => N 1 E x E
     | N _ l v r =>
-        if x ≤? v
-        then rebalance (insert x l) v r
-        else rebalance l v (insert x r)
+        if leb x v
+        then balance (insert leb x l) v r
+        else balance l v (insert leb x r)
 end.
 
-Lemma height_balance :
+Fixpoint fromList {A : Type} (leb : A -> A -> bool) (l : list A) : Tree A :=
+match l with
+    | [] => E
+    | h :: t => insert leb h (fromList leb t)
+end.
+
+Lemma height_prebalance :
   forall (A : Type) (v : A) (l r : Tree A),
-    height (balance l v r) = 1 + max (height l) (height r).
+    height (prebalance l v r) = 1 + max (height l) (height r).
 Proof.
   cbn. reflexivity.
 Qed.
 
 (* TODO: height_rotate *)
 
-Lemma height_rebalance :
+Lemma height_balance :
   forall (A : Type) (v : A) (l r : Tree A),
-    height (rebalance l v r) <= 1 + max (height l) (height r).
+    height (balance l v r) <= 1 + max (height l) (height r).
 Proof.
-  intros. functional induction @rebalance A l v r; trich; cbn in *.
+  intros. functional induction balance l v r; trich; cbn in *.
     destruct (height b).
       rewrite (@cmp_spec1 natlt) in e. cbn in e. lia.
       rewrite (@cmp_spec1 natlt) in e. cbn in e. lia.
@@ -72,9 +78,77 @@ Proof.
 Qed.
 
 Lemma height_insert :
-  forall (A : Ord) (x : A) (t : Tree A),
-    height (insert x t) <= 1 + height t.
+  forall {A : Type} (leb : A -> A -> bool) (x : A) (t : Tree A),
+    height (insert leb x t) <= 1 + height t.
 Proof.
-  intros. functional induction insert x t;
-  cbn; rewrite ?height_rebalance; lia.
+  intros.
+  functional induction insert leb x t;
+  cbn; rewrite ?height_balance; lia.
+Qed.
+
+(** Properties of [balance]. *)
+
+(* Lemma Elem_balance :
+  forall {A : Type} (c : color) (x v : A) (l r : RBTree A),
+    Elem x (N c l v r) <-> Elem x (balance c l v r).
+Proof.
+  split;
+  functional induction balance c l v r;
+  auto; intros; Elem'.
+Qed.
+ *)
+
+Lemma All_balance :
+  forall {A : Type} (P : A -> Prop) (v : A) (l r : Tree A),
+    All P (balance l v r) <-> All P l /\ P v /\ All P r.
+Proof.
+  intros.
+  functional induction balance l v r;
+  unfold prebalance;
+  firstorder All'.
+Qed.
+
+Lemma isBST2_balance :
+  forall (A : Ord) (h : nat) (v : A) (l r : Tree A),
+    isBST2 (N h l v r) -> isBST2 (balance l v r).
+Proof.
+  intros.
+  functional induction balance l v r;
+  isBST2'; unfold prebalance; clear e.
+    induction H4; isBST2'. trich.
+    induction H5; isBST2'. trich.
+Qed.
+
+(** Properties of [insert]. *)
+
+Lemma All_insert :
+  forall {A : Type} (P : A -> Prop) (leb : A -> A -> bool) (x : A) (t : Tree A),
+    All P (insert leb x t) <-> P x /\ All P t.
+Proof.
+  intros until t.
+  functional induction insert leb x t;
+  rewrite ?All_balance, ?IHt0;
+  firstorder All'.
+Qed.
+
+Lemma isBST2_insert :
+  forall {A : Ord} (x : A) (t : Tree A),
+    isBST2 t -> isBST2 (insert trich_leb x t).
+Proof.
+  intros until t.
+  functional induction insert trich_leb x t;
+  isBST2'.
+    apply isBST2_balance with 0. isBST2'. apply All_insert. split; trich.
+    apply isBST2_balance with 0. isBST2'. apply All_insert. split; trich.
+Qed.
+
+(** Properties of [fromList]. *)
+
+Lemma isBST2_fromList :
+  forall (A : Ord) (l : list A),
+    isBST2 (fromList trich_leb l).
+Proof.
+  induction l as [| h t]; cbn.
+    constructor.
+    apply isBST2_insert. assumption.
 Qed.
