Sorting/RedblackSort.v
@@ -1,41 +1,156 @@
-Require Export RedBlack.
 Require Import ListLemmas.
+Require Export RedBlack.
+Require Import Sorting.Sort.
 
-Fixpoint toList'_aux {A : Type} (t : RBTree A) (acc : list A) : list A :=
-match t with
-    | E => acc
-    | N _ l v r => toList'_aux l (v :: toList'_aux r acc)
-end.
+(** Sorting with red-black trees. *)
 
-Definition toList' {A : Type} (t : RBTree A) : list A := toList'_aux t [].
+Definition redblackSort
+  {A : Type} (leb : A -> A -> bool) (l : list A) : list A :=
+    toList (fromList leb l).
 
-Definition fromList' {A : Ord} (l : list A) : RBTree A :=
-  fold_left (fun t x => ins x t) l E.
+(** Sortedness properties *)
 
-Definition fromList'' {A : Ord} (l : list A) : RBTree A :=
-  fold_right (fun h t => ins h t) E l.
-
-Lemma toList'_aux_spec :
-  forall (A : Type) (t : RBTree A) (acc : list A),
-    toList'_aux t acc = toList t ++ acc.
+Lemma Sorted_toList :
+  forall (A : Ord) (t : RBTree A),
+    isBST t -> Sorted trich_le (toList t).
 Proof.
-  induction t; cbn; intros.
-    trivial.
-    rewrite IHt1, IHt2, <- app_assoc, <- app_comm_cons. trivial.
+  induction t as [| c l Hl v r Hr]; cbn; intros.
+    constructor.
+    inv H. apply Sorted_app_all; auto.
+      case_eq (toList r); intros; subst; auto. constructor.
+        apply H6. rewrite <- Elem_toList. rewrite H. cbn. auto.
+        rewrite <- H. auto.
+      intros. apply Elem_toList in H. auto.
 Qed.
 
-Theorem toList'_spec : @toList' = @toList color.
+Lemma Sorted_redblackSort :
+  forall (A : Ord) (l : list A),
+    Sorted trich_le (redblackSort trich_leb l).
 Proof.
-  ext A. ext t. unfold toList'.
-  rewrite toList'_aux_spec, app_nil_r. trivial.
+  intros. unfold redblackSort. apply Sorted_toList, isBST_fromList.
 Qed.
 
-#[refine]
+(** Permutation properties (proved directly). *)
+
+Lemma Permutation_toList_balance :
+  forall (A : Type) (c : color) (v : A) (l r : RBTree A),
+    Permutation (toList (balance c l v r)) (toList (N c l v r)).
+Proof.
+  intros.
+  functional induction balance c l v r;
+  cbn; rewrite <- ?app_assoc; cbn;
+  try reflexivity.
+    rewrite <- !app_assoc. cbn. reflexivity.
+Qed.
+
+Lemma Permutation_toList_ins :
+  forall {A : Type} (leb : A -> A -> bool) (x : A) (t : RBTree A),
+    Permutation (toList (ins leb x t)) (x :: toList t).
+Proof.
+  intros. functional induction ins leb x t.
+    cbn. reflexivity.
+    rewrite Permutation_toList_balance. cbn. rewrite IHr. cbn. reflexivity.
+    rewrite Permutation_toList_balance. cbn. rewrite IHr.
+      rewrite Permutation_middle. apply Permutation_app.
+        reflexivity.
+        constructor.
+Qed.
+
+Lemma Permutation_toList_insert :
+  forall {A : Type} (leb : A -> A -> bool) (x : A) (t : RBTree A),
+    Permutation (toList (insert leb x t)) (x :: toList t).
+Proof.
+  intros. unfold insert. destruct (ins leb x t) eqn: Heq; cbn.
+    apply (f_equal (Elem x)) in Heq. cut (@Elem color A x E).
+      inv 1.
+      rewrite <- Heq. rewrite Elem_ins. left. reflexivity.
+    rewrite <- (Permutation_toList_ins leb x t). rewrite Heq.
+      cbn. reflexivity.
+Qed.
+
+Lemma Permutation_redblackSort :
+  forall {A : Type} (leb : A -> A -> bool) (l : list A),
+    Permutation (redblackSort leb l) l.
+Proof.
+  intros. unfold redblackSort.
+  induction l as [| h t]; cbn.
+    reflexivity.
+    rewrite Permutation_toList_insert, IHt. reflexivity.
+Qed.
+
 Instance Sort_redblackSort (A : Ord) : Sort trich_le :=
 {
-    sort := @redblackSort A;
+    sort := redblackSort trich_leb;
     Sorted_sort := @Sorted_redblackSort A;
+    Permutation_sort := @Permutation_redblackSort A trich_leb;
 }.
+
+(** Permutation properties proved by way of counting. *)
+
+Lemma countEBT_balance :
+  forall (A : Type) (p : A -> bool) (c : color) (v : A) (l r : RBTree A),
+    countEBT p (balance c l v r) = countEBT p (N c l v r).
 Proof.
-  intros. apply perm_Permutation. rewrite <- perm_redblackSort. reflexivity.
-Defined.
+  intros.
+  functional induction balance c l v r;
+  cbn;
+  repeat match goal with
+      | |- context [if ?p then _ else _] => destruct p
+  end;
+  lia.
+Qed.
+
+Lemma countEBT_makeBlack :
+  forall (A : Type) (p : A -> bool) (t : RBTree A),
+    countEBT p (makeBlack t) = countEBT p t.
+Proof.
+  destruct t; reflexivity.
+Qed.
+
+Lemma countEBT_ins :
+  forall {A : Type} (leb : A -> A -> bool) (p : A -> bool) (x : A) (t : RBTree A),
+    countEBT p (ins leb x t) = (if p x then 1 else 0) + countEBT p t.
+Proof.
+  induction t; cbn;
+  try destruct (leb x a);
+  rewrite ?countEBT_balance; cbn; rewrite ?IHt1, ?IHt2;
+  repeat match goal with
+      | |- context [if ?p then _ else _] => destruct p
+  end;
+  lia.
+Qed.
+
+Lemma countEBT_insert :
+  forall {A : Type} (leb : A -> A -> bool) (p : A -> bool) (x : A) (t : RBTree A),
+    countEBT p (insert leb x t) = (if p x then 1 else 0) + countEBT p t.
+Proof.
+  intros. unfold insert.
+  rewrite countEBT_makeBlack, countEBT_ins. reflexivity.
+Qed.
+
+Lemma toList_countEBT :
+  forall (A : Type) (p : A -> bool) (t : RBTree A),
+    countEBT p t = count p (toList t).
+Proof.
+  induction t; cbn.
+    reflexivity.
+    rewrite count_app, IHt1, IHt2.
+      cbn. destruct (p a); lia.
+Qed.
+
+Lemma countEBT_fromList :
+  forall {A : Type} (leb : A -> A -> bool) (p : A -> bool) (l : list A),
+    countEBT p (fromList leb l) = count p l.
+Proof.
+  induction l as [| h t]; cbn; trich;
+  rewrite countEBT_insert, IHt.
+  destruct (p h); reflexivity.
+Qed.
+
+Lemma perm_redblackSort :
+  forall {A : Type} (leb : A -> A -> bool) (l : list A),
+    perm l (redblackSort leb l).
+Proof.
+  unfold perm, redblackSort. intros.
+  rewrite <- toList_countEBT, countEBT_fromList. reflexivity.
+Qed.
